\documentclass{article}
\usepackage{lipsum}
\usepackage{setspace}
\usepackage{nicematrix}
 \usepackage{relsize}
\NiceMatrixOptions{cell-space-limits=1pt}
 \onehalfspacing
\linespread{2}
\begin{document}

\[
\mathbf{d}_{QALY}=\begin{pNiceArray}{c}[small, baseline=line-3, first-row, first-col]
& \smaller \text{} \\
\smaller \text{H} & \texttt{uH}  \Delta_t\\
\smaller \text{S1} & \texttt{uS1}  \Delta_t\\
\smaller \text{S2} & \texttt{uS2}  \Delta_t\\ 
\smaller \text{DOC} & 0 \\
\smaller \text{DS} & 0 \\
\end{pNiceArray}
\]



\[
\mathbf{d}_{YLD}=\begin{pNiceArray}{c}[small, baseline=line-3, first-row, first-col]
& \smaller \text{} \\
\smaller \text{H} & 0  \\
\smaller \text{S1} & \texttt{dwS1} \frac{1}{r_{\Delta_t}}(1-e^{-r_{\Delta_t}}) \Delta_t\\
\smaller \text{S2} & \texttt{dwS2} \frac{1}{r_{\Delta_t}}(1-e^{-r_{\Delta_t}}) \Delta_t\\ 
\smaller \text{DOC} & 0 \\\
\smaller \text{DS} & 0 \\
\end{pNiceArray}
\]

\[
\mathbf{d}_{YLL,t}=\begin{pNiceArray}{c}[small, baseline=line-3, first-row, first-col]
& \smaller \text{} \\
\smaller \text{H} & 0  \\
\smaller \text{S1} & 0\\
\smaller \text{S2} & 0 \\
\smaller \text{D} & 0 \\\
\smaller \text{trDS} & \frac{1}{r}\big (1 - e^{-rEx(a_t)} \big )  \\
\end{pNiceArray}
\]

Let $S$ be an $\omega \times k$ matrix, $d$ be an $\omega \times k$ matrix, and $c$ be an $\omega \times 1$ vector.

The Hadamard product of $S$ and $d$ is given by:
\[ S \odot d = \begin{bmatrix}
s_{11}d_{11} & s_{12}d_{12} & \cdots & s_{1k}d_{1k} \\
s_{21}d_{21} & s_{22}d_{22} & \cdots & s_{2k}d_{2k} \\
\vdots & \vdots & \ddots & \vdots \\
s_{\omega 1}d_{\omega 1} & s_{\omega 2}d_{\omega 2} & \cdots & s_{\omega k}d_{\omega k}
\end{bmatrix} \]

Summing across the columns of $S \odot d$ to obtain a vector:
\[ \text{sum}(S \odot d) = \begin{bmatrix}
\sum_{j=1}^{k} s_{1j}d_{1j} \\
\sum_{j=1}^{k} s_{2j}d_{2j} \\
\vdots \\
\sum_{j=1}^{k} s_{\omega j}d_{\omega j}
\end{bmatrix} \]

Finally, performing the element-wise multiplication with vector $c$:
\[ \text{sum}(S \odot d) \odot c = \begin{bmatrix}
\left( \sum_{j=1}^{k} s_{1j}d_{1j} \right) c_1 \\
\left( \sum_{j=1}^{k} s_{2j}d_{2j} \right) c_2 \\
\vdots \\
\left( \sum_{j=1}^{k} s_{\omega j}d_{\omega j} \right) c_\omega
\end{bmatrix} \]



\end{document}